Add several examples of logic gen.

LogicGenerator/demo/implementation_1.v
@@ -1,15 +1,25 @@
 Require Import ZArith.
 
 Module NaiveLang.
-  Definition expr := (nat -> Z) -> Prop.
+  Definition expr := (nat -> option Z) -> Prop.
   Definition context := expr -> Prop.
   Definition impp (e1 e2 : expr) : expr := fun st => e1 st -> e2 st.
   Definition andp (e1 e2 : expr) : expr := fun st => e1 st /\ e2 st.
   Definition orp  (e1 e2 : expr) : expr := fun st => e1 st \/ e2 st.
   Definition falsep : expr := fun st => False.
-  Parameter sepcon : expr -> expr -> expr.
-  Parameter wand : expr -> expr -> expr.
-  Parameter emp : expr.
+
+  Definition join : (nat -> option Z) -> (nat -> option Z) -> (nat -> option Z) -> Prop :=
+    fun x y z =>
+      forall p: nat,
+       (exists v, x p = Some v /\ y p = None /\ z p = Some v) \/
+       (exists v, x p = None /\ y p = Some v /\ z p = Some v) \/
+       (x p = None /\ y p = None /\ z p = None).
+  Definition sepcon (e1 e2 : expr) : expr := fun st =>
+    exists st1 st2, join st1 st2 st /\ e1 st1 /\ e2 st2.
+  Definition wand (e1 e2 : expr) : expr := fun st =>
+    forall st1 st2, join st1 st2 st -> e1 st1 -> e2 st2.
+  Definition emp : expr := fun st =>
+    forall p, st p = None.
 
   Definition provable (e : expr) : Prop := forall st, e st.
 End NaiveLang.
