LogicGenerator/demo/configuration_2.v
@@ -1,0 +1,21 @@
+Require Import Coq.Lists.List.
+Require Import Logic.LogicGenerator.Utils.
+Require Import Logic.LogicGenerator.ConfigLang.
+
+Import ListNotations.
+
+Definition how_connectives :=
+  [primitive_connective impp
+  ;FROM_impp_TO_multi_imp
+  ].
+
+Definition how_judgements :=
+  [primitive_judgement provable
+  ].
+
+Definition transparent_names :=
+  [expr:parameter].
+
+Definition primitive_rule_classes :=
+  [ provability_OF_impp
+  ].
